fix the encode function

frodo/code/Hacl.Impl.Frodo.Encode.fst
@@ -45,12 +45,12 @@ let dc b c =
 inline_for_extraction noextract private
 val ec1:
     b:size_t{v b <= 8}
-  -> vij:uint64
+  -> x:uint64
   -> k:size_t{v k < 8}
-  -> res:uint16{res == S.ec1 (v b) vij (v k)}
-let ec1 b vij k =
-  FLemmas.modulo_pow2_u64 (vij >>. size_to_uint32 (b *! k)) (v b);
-  let rk = (vij >>. size_to_uint32 (b *! k)) &. ((u64 1 <<. size_to_uint32 b) -. u64 1) in
+  -> res:uint16{res == S.ec1 (v b) x (v k)}
+let ec1 b x k =
+  FLemmas.modulo_pow2_u64 (x >>. size_to_uint32 (b *! k)) (v b);
+  let rk = (x >>. size_to_uint32 (b *! k)) &. ((u64 1 <<. size_to_uint32 b) -. u64 1) in
   ec b (to_u16 rk)
 
 inline_for_extraction noextract private
@@ -58,29 +58,28 @@ val frodo_key_encode1:
     b:size_t{v b <= 8}
   -> a:lbytes (params_nbar *! params_nbar *! b /. size 8)
   -> res0:matrix_t params_nbar params_nbar
-  -> vij:uint64
+  -> vi:uint64
   -> i:size_t{v i < v params_nbar}
-  -> j:size_t{v j < v params_nbar / 8}
   -> Stack unit
     (requires fun h ->
       B.live h a /\ B.live h res0 /\ B.disjoint a res0)
     (ensures fun h0 _ h1 ->
       B.live h1 res0 /\ modifies (loc_buffer res0) h0 h1 /\
-      as_matrix h1 res0 == S.frodo_key_encode1 (v b) (B.as_seq h0 a) (as_matrix h0 res0) vij (v i) (v j))
-let frodo_key_encode1 b a res0 vij i j =
+      as_matrix h1 res0 == S.frodo_key_encode1 (v b) (B.as_seq h0 a) (as_matrix h0 res0) vi (v i))
+let frodo_key_encode1 b a res0 vi i =
   let h0 = ST.get () in
   Lib.Loops.for (size 0) (size 8)
   (fun h1 k ->
     B.live h1 res0 /\ B.live h1 a /\ modifies (loc_buffer res0) h0 h1 /\
-    (forall (i0:size_nat{i0 < v params_nbar /\ i0 <> v i}) (j:size_nat{j < v params_nbar / 8}) (k:size_nat{k < 8}).
-      get h1 res0 i0 (8 * j + k) == get h0 res0 i0 (8 * j + k)) /\
-    (forall (k1:size_nat{k1 < k}). get h1 res0 (v i) (8 * v j + k1) == S.ec1 (v b) vij k1) /\
-    (forall (k1:size_nat{k <= k1 /\ k1 < 8}). get h1 res0 (v i) (8 * v j + k1) == get h0 res0 (v i) (8 * v j + k1)))
+    (forall (i0:size_nat{i0 < v params_nbar /\ i0 <> v i}) (k:size_nat{k < 8}).
+      get h1 res0 i0 k == get h0 res0 i0 k) /\
+    (forall (k1:size_nat{k1 < k}). get h1 res0 (v i) k1 == S.ec1 (v b) vi k1) /\
+    (forall (k1:size_nat{k <= k1 /\ k1 < 8}). get h1 res0 (v i) k1 == get h0 res0 (v i) k1))
   (fun k ->
-    mset res0 i (size 8 *! j +! k) (ec1 b vij k)
+    mset res0 i k (ec1 b vi k)
   );
   let h2 = ST.get () in
-  S.lemma_matrix_equality_nbar (as_matrix h2 res0) (S.frodo_key_encode1 (v b) (B.as_seq h0 a) (as_matrix h0 res0) vij (v i) (v j))
+  S.lemma_matrix_equality_nbar (as_matrix h2 res0) (S.frodo_key_encode1 (v b) (B.as_seq h0 a) (as_matrix h0 res0) vi (v i))
 
 inline_for_extraction noextract private
 val frodo_key_encode2:
@@ -88,71 +87,22 @@ val frodo_key_encode2:
   -> a:lbytes (params_nbar *! params_nbar *! b /. size 8)
   -> res0:matrix_t params_nbar params_nbar
   -> i:size_t{v i < v params_nbar}
-  -> j:size_t{v j < v params_nbar / 8}
   -> Stack unit
     (requires fun h -> B.live h a /\ B.live h res0 /\ B.disjoint a res0)
     (ensures  fun h0 _ h1 ->
       B.live h1 a /\ B.live h1 res0 /\
       modifies (loc_buffer res0) h0 h1 /\
-      as_matrix h1 res0 == S.frodo_key_encode2 (v b) (B.as_seq h0 a) (as_matrix h0 res0) (v i) (v j))
-let frodo_key_encode2 b a res0 i j =
+      as_matrix h1 res0 == S.frodo_key_encode2 (v b) (B.as_seq h0 a) (as_matrix h0 res0) (v i))
+let frodo_key_encode2 b a res0 i =
   push_frame();
   let v8 = create (size 8) (u8 0) in
   let aLen = params_nbar *! params_nbar *! b /. size 8 in
-  update_sub v8 (size 0) b (sub #_ #_ #(v b) a ((i +! j) *! b) b);
-  let vij = uint_from_bytes_le #U64 v8 in
-  frodo_key_encode1 b a res0 vij i j;
+  update_sub v8 (size 0) b (sub #_ #_ #(v b) a (i *! b) b);
+  let vi = uint_from_bytes_le #U64 v8 in
+  frodo_key_encode1 b a res0 vi i;
   pop_frame()
 
-inline_for_extraction noextract private
-val frodo_key_encode_inner_inv:
-    h0:HS.mem
-  -> h1:HS.mem
-  -> h2:HS.mem
-  -> b:size_t{v b <= 8}
-  -> a:lbytes (params_nbar *! params_nbar *! b /. size 8)
-  -> res:matrix_t params_nbar params_nbar
-  -> i:size_t{v i < v params_nbar}
-  -> j:size_nat
-  -> Type0
-let frodo_key_encode_inner_inv h0 h1 h2 b a res i j =
-  let n2 = params_nbar /. size 8 in
-  j <= v n2 /\
-  B.live h2 res /\ B.live h2 a /\ B.disjoint a res /\
-  modifies (loc_buffer res) h1 h2 /\
-  (forall (i0:size_nat{i0 < v i}) (j:size_nat{j < v n2}) (k:size_nat{k < 8}). get h2 res i0 (8 * j + k) == get h1 res i0 (8 * j + k)) /\
-  (forall (j0:size_nat{j0 < j}) (k:size_nat{k < 8}). get h2 res (v i) (8 * j0 + k) == S.frodo_key_encode_inner (v b) (B.as_seq h0 a) (v i) j0 k) /\
-  (forall (j0:size_nat{j <= j0 /\ j0 < v n2}) (k:size_nat{k < 8}). get h2 res (v i) (8 * j0 + k) == get h0 res (v i) (8 * j0 + k)) /\
-  (forall (i0:size_nat{v i < i0 /\ i0 < v params_nbar}) (j:size_nat{j < v n2}) (k:size_nat{k < 8}). get h2 res i0 (8 * j + k) == get h0 res i0 (8 * j + k)) /\
-  B.as_seq h2 a == B.as_seq h0 a
-
-inline_for_extraction noextract private
-val frodo_key_encode_inner:
-    h0:HS.mem
-  -> h1:HS.mem
-  -> b:size_t{v b <= 8}
-  -> a:lbytes (params_nbar *! params_nbar *! b /. size 8)
-  -> res:matrix_t params_nbar params_nbar
-  -> i:size_t{v i < v params_nbar}
-  -> j:size_t{v j < v params_nbar / 8}
-  -> Stack unit
-    (requires fun h2 -> frodo_key_encode_inner_inv h0 h1 h2 b a res i (v j))
-    (ensures  fun _ _ h2 -> frodo_key_encode_inner_inv h0 h1 h2 b a res i (v j + 1))
-let frodo_key_encode_inner h0 h1 b a res i j =
-  assert (forall (k:size_nat{k < 8}).
-    M.mget (S.frodo_key_encode2 (v b) (B.as_seq h0 a) (as_matrix h0 res) (v i) (v j)) (v i) (8 * v j + k) ==
-    S.frodo_key_encode_inner (v b) (B.as_seq h0 a) (v i) (v j) k);
-  let h1 = ST.get () in
-  frodo_key_encode2 b a res i j;
-  let h2 = ST.get () in
-  assert (forall (k:size_nat{k < 8}). get h2 res (v i) (8 * v j + k) == S.frodo_key_encode_inner (v b) (B.as_seq h0 a) (v i) (v j) k)
-
-//TODO:move to Lemmas
-private
-val onemore: p:(nat -> Type0) -> q:(i:nat{p i} -> Type0) -> b:nat{p b} -> Lemma
-  (requires (forall (i:nat{p i /\ i < b}). q i) /\ q b)
-  (ensures  forall (i:nat{p i /\ i <= b}). q i)
-let onemore p q b = ()
+#set-options "--z3rlimit 50"
 
 val frodo_key_encode:
     b:size_t{v b <= 8}
@@ -165,68 +115,55 @@ val frodo_key_encode:
 [@"c_inline"]
 let frodo_key_encode b a res =
   push_frame();
-  let n2 = params_nbar /. size 8 in
 
   let h0 = ST.get () in
   Lib.Loops.for (size 0) params_nbar
   (fun h1 i ->
     B.live h1 res /\ modifies (loc_buffer res) h0 h1 /\
-    (forall (i0:size_nat{i0 < i}) (j:size_nat{j < v n2}) (k:size_nat{k < 8}).
-      get h1 res i0 (8 * j + k) == S.frodo_key_encode_inner (v b) (B.as_seq h0 a) i0 j k) /\
-    (forall (i0:size_nat{i <= i0 /\ i0 < v params_nbar}) (j:size_nat{j < v n2}) (k:size_nat{k < 8}).
-      get h1 res i0 (8 * j + k) == get h0 res i0 (8 * j + k)))
+    (forall (i0:size_nat{i0 < i}) (k:size_nat{k < 8}).
+      get h1 res i0 k == S.frodo_key_encode_inner (v b) (B.as_seq h0 a) i0 k) /\
+    (forall (i0:size_nat{i <= i0 /\ i0 < v params_nbar}) (k:size_nat{k < 8}).
+      get h1 res i0 k == get h0 res i0 k))
   (fun i ->
-    let h1 = ST.get () in
-    Lib.Loops.for (size 0) n2
-    (fun h2 j -> frodo_key_encode_inner_inv h0 h1 h2 b a res i j)
-    (fun j -> frodo_key_encode_inner h0 h1 b a res i j);
-    let h2 = ST.get () in
-    let q i1 = forall (j:size_nat{j < v n2}) (k:size_nat{k < 8}).
-      get h2 res i1 (8 * j + k) == S.frodo_key_encode_inner (v b) (B.as_seq h0 a) i1 j k in
-    onemore (fun i1 -> i1 < v params_nbar) q (v i)
+    frodo_key_encode2 b a res i
   );
   let h1 = ST.get () in
   S.lemma_matrix_equality_nbar (as_matrix h1 res) (S.frodo_key_encode (v b) (B.as_seq h0 a));
   pop_frame()
 
+
 val frodo_key_decode:
-  b:size_t{v b <= 8} ->
-  a:matrix_t params_nbar params_nbar ->
-  res:lbytes ((params_nbar *! params_nbar *! b) /. size 8) -> Stack unit
-  (requires (fun h -> B.live h a /\ B.live h res /\ B.disjoint a res))
-  (ensures (fun h0 r h1 -> B.live h1 res /\ modifies (loc_buffer res) h0 h1))
+    b:size_t{v b <= 8}
+  -> a:matrix_t params_nbar params_nbar
+  -> res:lbytes (params_nbar *! params_nbar *! b /. size 8)
+  -> Stack unit
+    (requires fun h -> B.live h a /\ B.live h res /\ B.disjoint a res)
+    (ensures  fun h0 r h1 -> B.live h1 res /\ modifies (loc_buffer res) h0 h1)
 [@"c_inline"]
 let frodo_key_decode b a res =
   push_frame();
-  let n2 = params_nbar /. size 8 in
-  let resLen = (params_nbar *! params_nbar *! b) /. size 8 in
+  let resLen = params_nbar *! params_nbar *! b /. size 8 in
+
   let v8 = create (size 8) (u8 0) in
   let templong:lbuffer uint64 1 = create (size 1) (u64 0) in
+
   let h0 = ST.get () in
   let inv (h1:mem) (j:nat{j <= v params_nbar}) =
     B.live h1 res /\ B.live h1 v8 /\ B.live h1 templong /\
     modifies (loc_union (loc_buffer res) (loc_union (loc_buffer v8) (loc_buffer templong))) h0 h1 in
   let f' (i:size_t{0 <= v i /\ v i < v params_nbar}): Stack unit
-      (requires (fun h -> inv h (v i)))
-      (ensures (fun _ _ h2 -> inv h2 (v i + 1))) =
-      let h0 = ST.get () in
-      let inv1 (h1:mem) (j:nat{j <= v n2}) =
-        B.live h1 res /\ B.live h1 v8 /\ B.live h1 templong /\
-        modifies (loc_union (loc_buffer res) (loc_union (loc_buffer v8) (loc_buffer templong))) h0 h1 in
-      let f1 (j:size_t{0 <= v j /\ v j < v n2}): Stack unit
-        (requires (fun h -> inv1 h (v j)))
-        (ensures (fun _ _ h2 -> inv1 h2 (v j + 1))) =
-          templong.(size 0) <- u64 0;
-          let h1 = ST.get () in
-          loop_nospec #h1 (size 8) templong
-          (fun k ->
-            let aijk = mget a i (size 8 *! j +! k) in
-            let aij = dc b aijk in
-            templong.(size 0) <- templong.(size 0) |. (to_u64 aij <<. size_to_uint32 (b *! k))
-          );
-          uint_to_bytes_le #U64 v8 (templong.(size 0));
-          copy (sub res ((i +! j) *! b) b) b (sub #uint8 #8 #(v b) v8 (size 0) b) in
+    (requires (fun h -> inv h (v i)))
+    (ensures (fun _ _ h2 -> inv h2 (v i + 1))) =
+      templong.(size 0) <- u64 0;
+      let h1 = ST.get () in
+      loop_nospec #h1 (size 8) templong
+      (fun k ->
+        let aijk = mget a i k in
+        let aij = dc b aijk in
+        templong.(size 0) <- templong.(size 0) |. (to_u64 aij <<. size_to_uint32 (b *! k))
+      );
+      uint_to_bytes_le #U64 v8 (templong.(size 0));
+      copy (sub res (i *! b) b) b (sub #uint8 #8 #(v b) v8 (size 0) b) in
 
-      Lib.Loops.for (size 0) n2 inv1 f1 in
   Lib.Loops.for (size 0) params_nbar inv f';
   pop_frame()
